src/Examples/ECC/Point.v
@@ -1,0 +1,36 @@
+Require Import Rupicola.Lib.Api.
+Require Import Rupicola.Examples.ECC.Field.
+
+Section Gallina.
+  Definition point : Type := (Z * Z).
+End Gallina.
+
+Section Compile.
+  Context {semantics : Semantics.parameters}
+          {semantics_ok : Semantics.parameters_ok semantics}.
+  Context {field_parameters : FieldParameters}
+          {bignum_representation : BignumRepresentation}.
+
+  Lemma compile_point_assign :
+    forall (locals: Semantics.locals) (mem: Semantics.mem)
+      tr R functions T (pred: T -> _ -> Prop)
+      (x y : Z) (X Y : bignum) k k_impl,
+      eval X = x ->
+      eval Y = y ->
+      let v := (x, y) in
+      (let head := v in
+       find k_impl
+            implementing (pred (dlet (eval X)
+                                     (fun x => dlet (eval Y)
+                                                    (fun y => k (x, y)))))
+       with-locals locals and-memory mem and-trace tr and-rest R
+       and-functions functions) ->
+      (let head := v in
+       find k_impl
+       implementing (pred (dlet head k))
+       with-locals locals and-memory mem and-trace tr and-rest R
+       and-functions functions).
+  Proof.
+    repeat straightline'. subst; auto.
+  Qed.
+End Compile.
